work more on append; add more features to CyclicBuffer, obtain write-access to the cells when incrementing the tail

concurrency/node-replication/CyclicBufferTokens.i.dfy
@@ -1,27 +1,67 @@
 include "../../lib/Lang/NativeTypes.s.dfy"
+include "InfiniteLogTokens.i.dfy"
+include "../framework/Cells.s.dfy"
+include "../framework/GlinearOption.s.dfy"
 
-module CyclicBufferTokens {
+module CyclicBufferTokens(nrifc: NRIfc) {
   import opened NativeTypes
+
+  import opened IL = InfiniteLogSSM(nrifc)
+  import opened ILT = InfiniteLogTokens(nrifc)
+  import opened GlinearOption
+  import opened Cells
 
   // Fixed number of replicas (in reference impl, this is variable)
   // TODO fill in reasonable constants for these
   const NUM_REPLICAS: uint64 := 4;
   const BUFFER_SIZE: uint64 := 9999;
 
-  // Use 'CB' prefix to distinguish these from the corresponding state in the InfiniteLog
-  // state machine.
+  datatype StoredType = StoredType(
+    cellContents: CellContents<LogEntry>,
+    logEntry: glOption<Log>
+  )
 
   // TODO add 'ghost loc' to these types
 
+  // Use 'CB' prefix to distinguish these from the corresponding state in the InfiniteLog
+  // state machine.
   datatype CBHead = CBHead(head: nat)
-
   datatype CBLocalTail = CBLocalTail(nodeId: nat, tail: nat)
-
   datatype CBGlobalTail = CBGlobalTail(tail: nat)
 
+  // The 'alive' bit flips back and forth. So sometimes 'true' means 'alive',
+  // and sometimes 'false' means 'alive'.
+  // entry is an index into the buffer (0 <= entry < BUFFER_SIZE)
+  datatype AliveBit = AliveBit(entry: nat, bit: bool)
+
+  // For advancing the head. We iterate idx from 0 .. NUM_REPLICAS and collect
+  // the min of all tails. Then we can set head to min_tail.
   datatype AdvanceHeadState = AdvanceHeadState(idx: nat, min_tail: nat)
 
+  // For advancing the tail and writing new log entries.
+  // First read the head, then advance the tail to some value allowed by the head.
+  // Then write the actual log entries.
   datatype AdvanceTailState = AdvanceTailState(observed_head: nat)
+  datatype AppendState = AppendState(cur_idx: nat, tail: nat)
+
+  // Contents stored in the log.
+  //
+  // `contents` maps an unbounded int to the resource protected there.
+  // The user of the CyclicBuffer state machine can thus maintain an invariant
+  // between the (unbounded) int and the resource.
+  //
+  // The way this is used is that the user, who is ready to write log-entry N,
+  //    * Advances the tail, obtaining access to buffer entry N % BUFFER_SIZE
+  //      which currently has entry N - BUFFER_SIZE
+  //    * They overwrite that entry with log entry N
+  //    * Return write-access to the CyclicBuffer protocol by setting the 'alive' bit
+  //
+  // Thus, for convenience, the `contents` needs to be initialized with
+  // -BUFFER_SIZE, ..., -1
+
+  datatype Contents = Contents(
+    contents: map<int, StoredType>
+  )
 
   glinear method init_advance_head_state(gshared first_local_tail: CBLocalTail)
   returns (glinear state': AdvanceHeadState)
@@ -47,9 +87,15 @@ module CyclicBufferTokens {
   ensures state'.observed_head == head.head
 
   glinear method finish_advance_tail(glinear state: AdvanceTailState, glinear tail: CBGlobalTail,
-      ghost new_tail: nat)
-  returns (glinear tail': CBGlobalTail)
+      ghost new_tail: nat, gshared contents: Contents)
+  returns (glinear tail': CBGlobalTail, glinear entries': map<nat, StoredType>,
+      glinear append': AppendState)
   requires tail.tail <= new_tail <= state.observed_head + BUFFER_SIZE as int
   ensures tail'.tail == new_tail
+  ensures forall i | tail.tail <= i < new_tail ::
+      && i in entries'
+      && i in contents.contents
+      && entries'[i] == contents.contents[i]
+  ensures append' == AppendState(tail.tail, new_tail)
 
 }
